***NO_CI*** more cleanup

examples/seplogic/FStar.SL.Monotonic.Heap.fst
@@ -228,37 +228,31 @@ let lemma_sel_equals_sel_tot_for_contained_refs #a #rel h r = ()
 let lemma_upd_equals_upd_tot_for_contained_refs #a #rel h r x = ()
 let lemma_modifies_and_equal_dom_sel_diff_addr #a #rel s h0 h1 r = ()
 
-let lemma_emp_with_next_addr_is_emp n = ()
-let lemma_r_unused_in_emp_with_next_addr #a #rel h r n= ()
-
-let lemma_r_unused_in_h #a #rel h r = ()
+let lemma_is_emp_emp_with_next_addr n = ()
+let lemma_get_next_addr_restrict #a #rel h r = ()
 let lemma_get_next_addr_points_to #a #rel r x = ()
-let lemma_get_next_addr_emp_next_addr n = ()
-
-let lemma_disjoint_points_to_unused_h #a #rel r x h1 = ()
-
-let lemma_join_tot_is_comm h1 h2 =
+let lemma_get_next_addr_emp_with_next_addr n = ()
+let lemma_r_unused_in_minus #a #rel h r = ()
+let lemma_r_unused_in_emp_with_next_addr #a #rel h r n = ()
+let lemma_r_unused_in_h #a #rel h r = ()
+let lemma_join_tot_is_comm h1 h2 = 
   assert (equal (join_tot h1 h2) (join_tot h2 h1))
-  
 let lemma_join_tot_restrict_minus #a #rel h r = 
-  assert (equal (join_tot (restrict h r) (minus h r)) (h))
-let lemma_join_tot_h_emp h =
-  assert (equal (join_tot h emp) h)
-let lemma_join_tot_emp_h h =
-  assert (equal (join_tot emp h) h)
-let lemma_join_tot_emp_with_next_addr_h h n =
+  assert (equal (join_tot (restrict h r) (minus h r)) h)
+let lemma_join_tot_emp_with_next_addr_h h n = 
   assert (equal (join_tot (emp_with_next_addr n) h) h)
-let lemma_join_tot_h_emp_with_next_addr h n =
+let lemma_join_tot_h_emp_with_next_addr h n = 
   assert (equal (join_tot h (emp_with_next_addr n)) h)
-
 let lemma_contains_r_join_tot_restrict_minus #a #rel h r = ()
 let lemma_contains_r1_join_tot_restrict_minus #a #rel h r r1 = ()
 let lemma_contains_r_join_tot_points_to_minus #a #rel h r x = ()
 let lemma_contains_r1_join_tot_points_to_minus #a #rel h r r1 x = ()
-let lemma_contains_join_tot_h_emp #a #rel h r = ()
 let lemma_contains_join_tot_h_emp_with_next_addr #a #rel h r n = ()
+let lemma_contains_join_tot_emp_with_next_addr_h #a #rel h r n = ()
 let lemma_contains_r_points_to_unused_h #a #rel r x h1 = ()
-
+let lemma_contains_r1_points_to_unused_h #a #rel r r1 x h1 = ()
+let lemma_contains_r_restrict_unused_h #a #rel h r h1 = ()
+let lemma_contains_r1_restrict_unused_h #a #rel h r r1 h1 = ()
 let lemma_restrict_r_join_tot_restrict_minus #a #rel h r =
   assert (equal (restrict (join_tot (restrict h r) (minus h r)) r) (restrict h r))
 let lemma_restrict_r1_join_tot_restrict_minus #a #rel h r r1 =
@@ -266,26 +260,21 @@ let lemma_restrict_r1_join_tot_restrict_minus #a #rel h r r1 =
 let lemma_restrict_r_join_tot_points_to_minus #a #rel h r x = 
   assert (equal (restrict (join_tot (points_to r x) (minus h r)) r) (points_to r x))
 let lemma_restrict_r1_join_tot_points_to_minus #a #rel h r r1 x =
-  assert (equal (restrict (join_tot (points_to r x) (minus h r)) r1) (restrict h r1))  
-let lemma_restrict_join_tot_h_emp #a #rel h r = 
-  assert (equal (restrict (join_tot h emp) r) (restrict h r))
+  assert (equal (restrict (join_tot (points_to r x) (minus h r)) r1) (restrict h r1))
 let lemma_restrict_join_tot_h_emp_with_next_addr #a #rel h r n = 
   assert (equal (restrict (join_tot h (emp_with_next_addr n)) r) (restrict h r))
-
+let lemma_restrict_join_tot_emp_with_next_addr_h #a #rel h r n =
+  assert (equal (restrict (join_tot (emp_with_next_addr n) h) r) (restrict h r))
 let lemma_sel_r_join_tot_restrict_minus #a #rel h r = ()
 let lemma_sel_r1_join_tot_restrict_minus #a #rel h r r1 = ()
 let lemma_sel_r_join_tot_points_to_minus #a #rel h r x = ()
 let lemma_sel_r1_join_tot_points_to_minus #a #rel h r r1 x = ()
-let lemma_sel_join_tot_h_emp #a #rel h r = ()
 let lemma_sel_join_tot_h_emp_with_next_addr #a #rel h r n = ()
-let lemma_sel_join_tot_emp_h #a #rel h r = ()
 let lemma_sel_join_tot_emp_with_next_addr_h #a #rel h r n = ()
-
 let lemma_restrict_eq_points_to #a #rel h r =
   let h1 = restrict h r in
   let Some (| _, _, _, _ |) = h1.memory r.addr in
   ()
-
 let lemma_points_to_is_injective #a #rel r x y = 
   assert (sel (points_to r x) r == sel (points_to r y) r)
 
