examples/seplogic/Examples.fst
@@ -1,11 +1,12 @@
-module Examples
+module Test
 
 open Lang
-open FStar.SepLogic.Heap
+
+open FStar.SL.Heap
 
 open FStar.Tactics
 
-#reset-options "--log_queries --using_facts_from '* -FStar.Tactics -FStar.Reflection'"
+#reset-options "--using_facts_from '* -FStar.Tactics -FStar.Reflection'"
 
 let unfold_fns :list string = [
   "wp_command";
@@ -27,135 +28,6 @@ let unfold_fns :list string = [
 unfold let unfold_steps =
   List.Tot.map (fun s -> "Lang." ^ s) unfold_fns
 
-let step_alloc_return :tactic unit =
-  dump "In step_alloc_return";;
-  apply_lemma (quote lemma_alloc_return);; norm [];;
-  dump "After step_alloc_return"
-
-let step_bind :tactic unit = 
-  dump "In step_bind";;
-  apply_lemma (quote lemma_bind);; norm [];;
-  dump "After step_bind"
-
-let step_eq_implies_intro :tactic unit =
-  dump "In step_eq_implies_intro";;
-  apply_lemma (quote lemma_eq_implies_intro);; norm [];;
-  dump "After step_eq_implies_intro"
-
-// let step_extract_disjoint :tactic unit =
-//   dump "In step_extract_disjoint";;
-//   apply_lemma (quote lemma_extract_disjoint);; norm [];;
-//   dump "After lemma_extract_disjoint"
-//   // split;;
-//   // dump "After split";;
-//   // // TODO - Replace "smt" with "simplify_disjoint"
-//   // smt
-
-let assumption'  :tactic unit = 
-  apply_raw (quote FStar.Squash.return_squash);; assumption
-
-let assumption'' :tactic unit = 
-  or_else assumption' (apply_lemma (quote lemma_addr_not_eq_refl);; norm [];; assumption')
-
-let step_read_write       :tactic unit = 
-  dump "In step_read_write";;
-  apply_lemma (quote lemma_read_write);; norm [];;
-  dump "After lemma_read_write"
-  // split;;
-  // dump "After split";;
-  // // TODO - Replace "smt" with "simplify_contains"
-  // smt
-
-let step_restrict :tactic unit =
-  dump "In step_restrict";;
-  (apply_lemma (quote lemma_restrict_r_join_points_to_minus')) `or_else`
-  (apply_lemma (quote lemma_restrict_r1_join_points_to_minus');; assumption'')
-       
-  // or_else (apply_lemma (quote lemma_restrict_r_join_restrict_minus);;
-  //          // TODO - Replace "smt" with "simplify_contains"
-  //          smt)
-  //         (apply_lemma (quote lemma_restrict_r1_join_restrict_minus);;
-  // 	   repeat (split);; 
-  // 	   // TODO - Replace "smt" with "simplify_contains"
-  // 	   smt;; 
-  // 	   smt;; 
-  // 	   assumption'')
-
-let simplify_restrict :tactic unit =
-  apply_lemma (quote lemma_eq_l_cong);;
-  step_restrict;;
-  trytac trefl;;
-  return ()
-
-let simplify_join_emp :tactic unit =
-  dump "In simplify_join_emp";;
-  pointwise (or_else (or_else (apply_lemma (quote lemma_join_h_emp');; qed) 
-                              (apply_lemma (quote lemma_join_emp_h');; qed))
-		     (fail "SKIP"))
-
-let simplify_join_minus :tactic unit =
-  dump "In simplify_join_minus";;
-  pointwise (or_else (apply_lemma (quote lemma_join_restrict_minus');; qed)
-		     (fail "SKIP"))
-
-  // pointwise (or_else (apply_lemma (quote lemma_join_restrict_minus);;
-  //                     // TODO - Replace "smt" with "simplify_contains"
-  // 		      smt)
-  // 		     (fail "SKIP"))
-
-// let step_disjoint :tactic unit =
-//   dump "In step_disjoint";;
-//   split;;
-//   dump "After split";;
-//   // TODO - Replace "smt" with "step_disjoint"
-//   smt
-
-let simplify_join :tactic unit =
-  dump "In simplify_join";;
-  apply_lemma (quote lemma_impl_l_cong);;
-  simplify_join_emp;;
-  simplify_join_minus;;
-  dump "After simplify_join_minus";;
-  apply_lemma (quote lemma_refl)
-
-let step_intros :tactic unit =
-  dump "In step_intros";;
-  forall_intros;;
-  simplify_join;;
-  repeat simplify_restrict;;
-  implies_intro;;
-  return ()
-
-let step :tactic unit =
-  dump "In step";;
-  step_bind                   `or_else`
-  step_read_write             `or_else`
-  step_alloc_return           `or_else`
-  step_eq_implies_intro       `or_else`
-  step_intros                 `or_else`
-  // step_extract_disjoint       `or_else`
-  // step_disjoint               `or_else`
-  fail "step: failed"
-
-let step_sel :tactic unit =
-  dump "In step_sel";;
-  // (apply_lemma (quote lemma_sel_r_join_points_to_minus);; 
-  //  // TODO - Replace "smt" with "simplify_contains"
-  //  smt)           `or_else`
-  (apply_lemma (quote lemma_sel_r_join_points_to_minus'))                        `or_else`
-  (apply_lemma (quote lemma_sel_r1_join_points_to_minus');; assumption'')        `or_else`
-  (apply_lemma (quote lemma_sel_r1_from_restrict');; dump "ss3";;  assumption'') `or_else`
-  (apply_lemma (quote lemma_sel_r_from_minus');; dump "ss4";; assumption'')      `or_else`
-  fail "step_sel: failed"
-
-let simplify_sel :tactic unit =
-  dump "In simplify_sel";;
-  trytac (apply_lemma (quote lemma_eq_cong);; norm []);;
-  step_sel;;
-  dump "After step_sel";;
-  trytac trefl;;
-  return ()
-
 let and_elim' :tactic unit =
   h <-- implies_intro;
   and_elim (pack (Tv_Var h));;
@@ -166,172 +38,155 @@ let implies_intros' :tactic unit =
   implies_intros;;
   return ()
 
-let rec repeat_simplify_sel () :Tac unit =
+let assumption'  :tactic unit = 
+  apply_raw (quote FStar.Squash.return_squash);; assumption
+
+let assumption'' :tactic unit = 
+  or_else assumption' (apply_lemma (quote lemma_addr_not_eq_refl);; norm [];; assumption')
+
+let rec split_all () :Tac unit =
+  ( g <-- cur_goal;
+    match (term_as_formula g) with
+    | And _ _ -> split;; iseq [split_all; split_all]
+    | _       -> return ()
+  ) ()
+
+(***** Tactics *****)
+
+let simplify_unused_in :tactic unit =
+  apply_lemma (quote lemma_r_unused_in_minus) `or_else`
+  apply_lemma (quote lemma_r_unused_in_h)     `or_else`
+  return ()
+
+let simplify_contains_aux :tactic unit =
+  assumption'' `or_else`
+  apply_lemma (quote lemma_contains_r_join_tot_restrict_minus)     `or_else`
+  apply_lemma (quote lemma_contains_r_join_tot_points_to_minus)    `or_else`
+  apply_lemma (quote lemma_contains_r1_join_tot_restrict_minus)    `or_else`
+  apply_lemma (quote lemma_contains_r1_join_tot_points_to_minus)   `or_else`
+  apply_lemma (quote lemma_contains_join_tot_h_emp_with_next_addr) `or_else`
+  apply_lemma (quote lemma_contains_r_points_to_unused_h);;
+  split_all;;
+  simplify_unused_in;;
+  norm []
+
+let simplify_contains :tactic unit =
+  repeat simplify_contains_aux;;
+  return ()
+
+let simplify_restrict_aux :tactic unit =
+  apply_lemma (quote lemma_eq_l_cong);; 
+  norm [];;
+  apply_lemma (quote lemma_restrict_r_join_tot_points_to_minus)  `or_else`
+  apply_lemma (quote lemma_restrict_r_join_tot_restrict_minus)   `or_else`
+  apply_lemma (quote lemma_restrict_r1_join_tot_restrict_minus)  `or_else`
+  apply_lemma (quote lemma_restrict_r1_join_tot_points_to_minus) `or_else`
+  apply_lemma (quote lemma_restrict_join_tot_h_emp_with_next_addr);;
+  norm [];;
+  simplify_contains
+
+let simplify_restrict :tactic unit =
+  repeat simplify_restrict_aux;;
+  trytac trefl;;
+  return ()
+
+let step_bind :tactic unit = 
+  apply_lemma (quote lemma_bind);;
+  norm []
+
+let step_read_write :tactic unit = 
+  apply_lemma (quote lemma_read_write);;
+  norm [];;
+  simplify_contains
+
+let step_alloc_return :tactic unit =
+  apply_lemma (quote lemma_alloc_return);;
+  norm [];;
+  simplify_contains
+
+let step_eq_implies_intro :tactic unit =
+  apply_lemma (quote lemma_eq_implies_intro);;
+  norm []
+
+let step_eq_implies_intro' :tactic unit =
+  forall_intro;;
+  apply_lemma (quote lemma_eq_implies_intro');;
+  norm [];;
+  implies_intro;;
+  return ()
+
+let step_intro :tactic unit =
+  norm [];;
+  forall_intro;;
+  simplify_restrict;;
+  implies_intro;;
+  return ()
+
+let step :tactic unit =
+  step_bind              `or_else`
+  step_read_write        `or_else`
+  step_alloc_return      `or_else`
+  step_eq_implies_intro  `or_else`
+  step_eq_implies_intro' `or_else`
+  step_intro             `or_else`
+  fail "step: failed"
+
+let simplify_select :tactic unit =
+ apply_lemma (quote lemma_sel_r_join_tot_restrict_minus)     `or_else`
+ apply_lemma (quote lemma_sel_r_join_tot_points_to_minus)    `or_else`
+ apply_lemma (quote lemma_sel_r1_join_tot_restrict_minus)    `or_else`
+ apply_lemma (quote lemma_sel_r1_join_tot_points_to_minus)   `or_else`
+ apply_lemma (quote lemma_sel_join_tot_h_emp_with_next_addr) `or_else`
+ apply_lemma (quote lemma_sel_join_tot_emp_with_next_addr_h);;
+ simplify_contains
+
+let step_select :tactic unit =
+ apply_lemma (quote lemma_eq_cong);; 
+ norm [];;
+ simplify_select;;
+ trytac trefl;;
+ return ()
+
+let rec repeat_step_select () :Tac unit =
   (g <-- trytac cur_goal;
   begin match g with
   | None -> return ()
-  | Some _ -> repeat simplify_sel;;
-              dump "After repeat simplify_sel";;
+  | Some _ -> repeat step_select;;
               trytac ((trefl;; qed) `or_else` smt);;
-              repeat_simplify_sel
+              repeat_step_select
   end
   ) ()
 
-let simplify_goals :tactic unit =
-  dump "In simplify_goals";;
-  simplify_join_emp;;
-  dump "After simplify_join_emp";;
-  simplify_join_minus;;
-  dump "After simplify_join_minus";;
-  trytac (repeat split);;
-  dump "After trytac (repeat split)";;
-  repeat_simplify_sel;;
-  dump "After repeat_simplify_sel";;
-  return ()
+let simplify :tactic unit =
+ split_all;;
+ repeat_step_select;;
+ return ()
 
 let solve :tactic unit =
-  norm [delta; delta_only unfold_steps; primops];;
-  dump "Initial goal";;
-  trytac implies_intros';;
-  e <-- cur_env;
-  rewrite_all_context_equalities (binders_of_env e);;
-  dump "After trytac implies_intros'";;
-  repeat step;;
-  dump "After repeat step";;
-  simplify_goals;;
-  dump "After simplify_goals";;
-  dump "Final goal"
+ norm [delta; delta_only unfold_steps; primops];;
+ trytac implies_intros';;
+ dump "Initial goal";;
+ repeat step;;
+ simplify;;
+ dump "Final goal"
 
-let norm_step: tactic unit =
-  norm [delta; delta_only unfold_steps; primops];;
-  return ()
-  
 (***** Examples *****)
 open FStar.UInt
 open FStar.UInt64
 
 type t = UInt64.t
 
-// let write_ok (h:heap) (r:addr) (n:t) =
-//   let c = (Write r n) in
-//   let p = fun _ h -> sel h r == n in
-//   let post = (lift_wpsep (wpsep_command c)) p h in
-//   assert_by_tactic (h `contains` r ==> post) (
-//     norm [delta; delta_only unfold_steps; primops];;
-//     implies_intros';;
-//     apply_lemma (quote lemma_read_write);;
-//     norm [];;
-//     split;;
-//     assumption'';;
-//     apply_lemma (quote lemma_eq_implies_intro);;
-//     norm [];;
-//     split;;
-//     apply_lemma (quote lemma_disjoint_points_to_minus);;
-//     norm [];;
-//     assumption'';;
-//     apply_lemma (quote lemma_sel_r_join_points_to_minus);;
-//     norm [];;
-//     assumption''
-//   )
-
 let write_ok (h:heap) (r:addr) (n:t) =
   let c = (Write r n) in
   let p = fun _ h -> sel h r == n in
   let post = (lift_wpsep (wpsep_command c)) p h in
   assert_by_tactic (h `contains` r ==> post) solve
-
-// let increment_ok (h:heap) (r:addr) (n:t) =
-//   let c = Bind (Read r) (fun n -> Write r (n +?^ 1uL)) in
-//   let p = fun _ h -> (sel h r == n +?^ 1uL) in
-//   let post = (lift_wpsep (wpsep_command c)) p h in
-//   assert_by_tactic (h `contains` r /\ sel h r == n ==> post) (
-//     norm [delta; delta_only unfold_steps; primops];;
-//     implies_intros';;
-//     apply_lemma (quote lemma_bind);;
-//     norm [];;
-//     apply_lemma (quote lemma_read_write);;
-//     norm [];;
-//     split;;
-//     assumption'';;
-//     forall_intro;;
-//     implies_intro;;
-//     apply_lemma (quote lemma_extract_disjoint);;
-//     norm [];;
-//     split;;
-//     apply_lemma (quote lemma_disjoint_restrict_minus);;
-//     norm [];;
-//     assumption'';;
-//     apply_lemma (quote lemma_read_write);;
-//     norm [];;
-//     split;;
-//     smt;;
-//     apply_lemma (quote lemma_eq_implies_intro);;
-//     norm [];;
-//     split;;
-//     apply_lemma (quote lemma_disjoint_points_to_minus);;
-//     norm [];;
-//     smt;;
-//     split;;
-//     apply_lemma (quote lemma_emp_disjoint);;
-//     norm [];;
-//     apply_lemma (quote lemma_eq_cong);;
-//     norm [];;
-//     apply_lemma (quote lemma_sel_join_h_emp);;
-//     norm [];;
-//     apply_lemma (quote lemma_eq_cong);;
-//     norm [];;
-//     apply_lemma (quote lemma_sel_r_join_points_to_minus);;
-//     norm [];;
-//     smt
-//   )
-
+  
 let increment_ok (h:heap) (r:addr) (n:t) =
   let c = Bind (Read r) (fun n -> Write r (n +?^ 1uL)) in
   let p = fun _ h -> (sel h r == n +?^ 1uL) in
   let post = (lift_wpsep (wpsep_command c)) p h in
   assert_by_tactic (h `contains` r /\ sel h r == n ==> post) solve
- 
-// let swap_ok (r1:addr) (r2:addr) (h:heap) (a:t) (b:t) =
-//   let c = Bind (Read r1) (fun n1 -> Bind (Read r2) (fun n2 -> Bind (Write r1 n2) (fun _ -> Write r2 n1))) in
-//   let p = fun _ h -> (sel h r1 == b /\ sel h r2 == a) in
-//   let post = (lift_wpsep (wpsep_command c)) p h in
-//   assert_by_tactic (h `contains` r1 /\  h `contains` r2 /\ addr_of r1 <> addr_of r2 /\ sel h r1 == a /\ sel h r2 == b ==> post) (
-//     norm [delta; delta_only unfold_steps; primops];;
-//     implies_intros';;
-//     apply_lemma (quote lemma_bind);;
-//     norm [];;
-//     apply_lemma (quote lemma_read_write);;
-//     norm [];;
-//     split;;
-//     assumption'';;
-//     forall_intro;;
-//     implies_intro;;
-//     apply_lemma (quote lemma_extract_disjoint);;
-//     norm [];;
-//     split;;
-//     smt;;
-//     apply_lemma (quote lemma_bind);;
-//     norm [];;
-//     apply_lemma (quote lemma_read_write);;
-//     norm [];;
-//     split;;
-//     smt;;
-//     forall_intro;;
-//     apply_lemma (quote lemma_eq_l_cong);;
-//     norm [];;
-//     apply_lemma (quote lemma_restrict_r1_join_restrict_minus);;
-//     norm [];;
-//     repeat (split);;
-//     assumption'';;
-//     assumption'';;
-//     assumption'';;
-//     implies_intro;;
-//     apply_lemma (quote lemma_extract_disjoint);;
-//     norm [];;
-//     apply_lemma (quote lemma_read_write);;
-//     norm [];;
-//     fail "here"
-//   )
 
 let swap_ok (r1:addr) (r2:addr) (h:heap) (a:t) (b:t) =
   let c = Bind (Read r1) (fun n1 -> Bind (Read r2) (fun n2 -> Bind (Write r1 n2) (fun _ -> Write r2 n1))) in
@@ -345,22 +200,22 @@ let double_increment_ok (r:addr) (h:heap) (n:t{size (v n + 2) FStar.UInt64.n}) =
   let t = (lift_wpsep (wpsep_command c)) p h in
   assert_by_tactic (h `contains` r /\ sel h r == n ==> t) solve
 
-let rotate_ok (r1:addr) (r2:addr) (r3:addr) (h:heap) (i:t) (j:t) (k:t) =
-  let c = Bind (Bind (Read r1) (fun n1 -> Bind (Read r2) (fun n2 -> Bind (Write r1 n2) (fun _ -> Write r2 n1)))) (fun _ -> Bind (Read r2) (fun n3 -> Bind (Read r3) (fun n4 -> Bind (Write r2 n4) (fun _ -> Write r3 n3)))) in
-  let p = fun _ h -> (sel h r1 == j /\ sel h r2 == k /\ sel h r3 == i) in
-  let t = (lift_wpsep (wpsep_command c)) p h in
-  assert_by_tactic (h `contains` r1 /\ h `contains` r2 /\ h `contains` r3 /\ 
-                    addr_of r1 <> addr_of r2 /\ addr_of r2 <> addr_of r3 /\ addr_of r1 <> addr_of r3 /\
-		    sel h r1 == i /\ sel h r2 == j /\ sel h r3 == k ==> t) solve
+// let rotate_ok (r1:addr) (r2:addr) (r3:addr) (h:heap) (i:t) (j:t) (k:t) =
+//   let c = Bind (Bind (Read r1) (fun n1 -> Bind (Read r2) (fun n2 -> Bind (Write r1 n2) (fun _ -> Write r2 n1)))) (fun _ -> Bind (Read r2) (fun n3 -> Bind (Read r3) (fun n4 -> Bind (Write r2 n4) (fun _ -> Write r3 n3)))) in
+//   let p = fun _ h -> (sel h r1 == j /\ sel h r2 == k /\ sel h r3 == i) in
+//   let t = (lift_wpsep (wpsep_command c)) p h in
+//   assert_by_tactic (h `contains` r1 /\ h `contains` r2 /\ h `contains` r3 /\ 
+//                     addr_of r1 <> addr_of r2 /\ addr_of r2 <> addr_of r3 /\ addr_of r1 <> addr_of r3 /\
+// 		    sel h r1 == i /\ sel h r2 == j /\ sel h r3 == k ==> t) solve
 
 let init_ok (h:heap) =
   let c = Bind (Alloc) (fun (r1:addr) -> Bind (Write r1 7uL) (fun _ -> Return r1)) in
   let p = fun r h -> sel h r == 7uL in
   let t = (lift_wpsep (wpsep_command c)) p h in
-  assert_by_tactic t solve 
+  assert_by_tactic t solve
 
 let copy_ok (r1:addr) (r2:addr) (r3:addr) (h:heap) (i:t) (j:t) (k:t) =
   let c = Bind (Read r1) (fun n1 -> Write r2 (n1)) in
   let p = fun _ h -> (sel h r1 == i /\ sel h r2 == i /\ sel h r3 == k) in
   let post = (lift_wpsep (wpsep_command c)) p h in
-  assert_by_tactic (addr_of r1 <> addr_of r2 /\ addr_of r2 <> addr_of r3 /\ addr_of r1 <> addr_of r3 /\ sel h r1 == i /\ sel h r2 == j /\ sel h r3 == k ==> post) solve //here how can we apply a binder?
+  assert_by_tactic (h `contains` r1 /\ h `contains` r2 /\ h `contains` r3 /\ addr_of r1 <> addr_of r2 /\ addr_of r2 <> addr_of r3 /\ addr_of r1 <> addr_of r3 /\ sel h r1 == i /\ sel h r2 == j /\ sel h r3 == k ==> post) solve
